common/Memtype.v
@@ -617,10 +617,13 @@ Class MemoryModel mem `{memory_model_ops: MemoryModelOps mem}
   \/ (b' <> b \/ ofs' + size_chunk chunk' <= ofs \/ ofs + size_chunk chunk <= ofs');
 
  store_same_ptr:
-   forall m1 b1 o1 b o m2,
-     load Mptr m1 b1 o1 = Some (Vptr b o) ->
-     store Mptr m1 b1 o1 (Vptr b o) = Some m2 -> m1 = m2;
+   forall m1 b o v m2,
+     v <> Vundef ->
+     Val.has_type v Tptr ->
+     loadbytes m1 b o (size_chunk Mptr) = Some (encode_val Mptr v) ->
+     store Mptr m1 b o v = Some m2 -> m1 = m2;
 
+ 
 (** Load-store properties for [loadbytes]. *)
 
  loadbytes_store_same:
@@ -3112,15 +3115,6 @@ Qed.
     - eapply record_stack_block_perm'. eauto.
       eapply perm_alloc_1. eauto.
       eapply push_new_stage_perm. auto.
-  Qed.
-
-  Lemma storev_same_ptr:
-   forall m1 addr b o m2,
-     loadv Mptr m1 addr = Some (Vptr b o) ->
-     storev Mptr m1 addr (Vptr b o) = Some m2 -> m1 = m2.
-  Proof.
-    unfold loadv, storev. intros. repeat destr_in H.
-    eapply store_same_ptr; eauto.
   Qed.
 
 End WITHMEMORYMODEL.
